Some experiments into reification

coq/theories/automation/AutomationLemmas.v
@@ -2,16 +2,22 @@ Require Import impboot.functional.FunSyntax.
 Require Import impboot.functional.FunSemantics.
 Require Import impboot.functional.FunProperties.
 Require Import impboot.functional.FunValues.
+Require impboot.imperative.ImpSyntax.
 From impboot Require Import utils.Core.
+From coqutil Require Import dlet.
+Require Import impboot.utils.Words4Naive.
+Require Import coqutil.Word.Interface.
+Require Import coqutil.Word.Naive.
+Require Import impboot.utils.AppList.
 
 Create HintDb automation.
 
 Theorem trans_app: forall n params vs b body s s1 v,
   let env := make_env params vs Env.empty in
-    (b -> (env |- ([body], s) ---> ([v], s1))) ->
+    (b -> (env |-- ([body], s) ---> ([v], s1))) ->
     List.length params = List.length vs ->
-    lookup_fun (value_name n) s.(funs) = Some (params,body) ->
-    b -> eval_app (value_name n) vs s (v,s1).
+    lookup_fun (name_enc n) s.(funs) = Some (params,body) ->
+    b -> eval_app (name_enc n) vs s (v,s1).
 Proof.
   intros; eapply App_intro; eauto.
   unfold env_and_body; simpl.
@@ -21,9 +27,9 @@ Proof.
 Qed.
 
 Theorem trans_Call : forall b1 b2 env xs s1 s2 s3 fname vs v,
-  (b1 -> env |- (xs, s1) ---> (vs, s2)) ->
+  (b1 -> env |-- (xs, s1) ---> (vs, s2)) ->
   (b2 -> eval_app fname vs s2 (v, s3)) ->
-  (b1 /\ b2 -> env |- ([Call fname xs], s1) ---> ([v], s3)).
+  (b1 /\ b2 -> env |-- ([Call fname xs], s1) ---> ([v], s3)).
 Proof.
   intros b1 b2 env xs s1 s2 s3 fname vs v H1 H2 [Hb1 Hb2].
   apply H1 in Hb1; apply H2 in Hb2.
@@ -32,24 +38,24 @@ Proof.
 Qed.
 
 Theorem trans_Var : forall n v env s,
-  Env.lookup env (value_name n) = Some v ->
-  env |- ([Var (value_name n)], s) ---> ([v], s).
+  Env.lookup env (name_enc n) = Some v ->
+  env |-- ([Var (name_enc n)], s) ---> ([v], s).
 Proof.
   intros n v env s H.
   apply Eval_Var; auto.
 Qed.
 
 Theorem trans_nil : forall env s,
-  env |- ([], s) ---> ([], s).
+  env |-- ([], s) ---> ([], s).
 Proof.
   intros env s.
   apply Eval_Nil.
 Qed.
 
 Theorem trans_cons : forall x xs v vs env s s1 s2,
-  env |- ([x], s) ---> ([v], s1) ->
-  env |- (xs, s1) ---> (vs, s2) ->
-  env |- (x :: xs, s) ---> (v :: vs, s2).
+  env |-- ([x], s) ---> ([v], s1) ->
+  env |-- (xs, s1) ---> (vs, s2) ->
+  env |-- (x :: xs, s) ---> (v :: vs, s2).
 Proof.
   intros x xs v vs env s s1 s2 H1 H2.
   destruct xs; simpl in *.
@@ -57,46 +63,6 @@ Proof.
     assumption.
   - inversion H2; subst; econstructor; eauto.
 Qed.
-
-(* TODO(kπ) letd? *)
-Theorem auto_let : forall {A B} `{ra : Refinable A} `{rb : Refinable B}
-    b1 b2 env x1 y1 s1 s2 s3 v1 let_n f,
-  (b1 -> env |- ([x1], s1) ---> ([ra.(refine) v1], s2)) ->
-  (forall v1, b2 v1 -> (Env.insert ((value_name let_n), Some (ra.(refine) v1)) env) |- ([y1], s2) ---> ([rb.(refine) (f v1)], s3)) ->
-  (b1 /\ b2 v1 ->
-    env |- ([Let (value_name let_n) x1 y1], s1) ---> ([rb.(refine) (f v1)], s3)).
-Proof.
-  intros.
-  destruct H1.
-  eapply Eval_Let; eauto.
-Qed.
-
-Theorem auto_otherwise : forall {A} `{ra : Refinable A}
-    b1 env s x1 v1,
-  (b1 -> env |- ([x1], s) ---> ([refine v1], s)) ->
-  (b1 ->
-    env |- ([If Less [Const 0; Const 1] x1 (Const 0)], s) ---> ([refine (value_otherwise v1)], s)).
-Proof.
-  intros.
-  apply H in X.
-  repeat econstructor; eauto.
-Qed.
-
-(* bool *)
-
-Theorem auto_bool_F : forall env s,
-  env |- ([Const 0], s) ---> ([refine false], s).
-Proof.
-  intros. apply Eval_Const.
-Qed.
-Hint Resolve auto_bool_F : automation.
-
-Theorem auto_bool_T : forall env s,
-  env |- ([Const 1], s) ---> ([refine true], s).
-Proof.
-  intros. apply Eval_Const.
-Qed.
-Hint Resolve auto_bool_T : automation.
 
 Ltac Eval_eq :=
   repeat match goal with
@@ -107,9 +73,51 @@ Ltac Eval_eq :=
   | _ => eauto
   end.
 
+Theorem auto_let : forall {A B} `{ra : Refinable A} `{rb : Refinable B}
+    b1 b2 env x1 y1 s1 s2 s3 v1 let_n f,
+  (b1 -> env |-- ([x1], s1) ---> ([ra.(encode) v1], s2)) ->
+  (forall v1, b2 v1 -> (Env.insert ((name_enc let_n), Some (ra.(encode) v1)) env) |-- ([y1], s2) --->
+                       ([rb.(encode) (f v1)], s3)) ->
+  (b1 /\ b2 v1 ->
+    env |-- ([Let (name_enc let_n) x1 y1], s1) ---> ([rb.(encode) (dlet v1 f)], s3)).
+Proof.
+  intros.
+  destruct H1.
+  eapply Eval_Let; eauto.
+Qed.
+Hint Resolve auto_let : automation.
+
+Theorem auto_otherwise : forall {A} `{ra : Refinable A}
+    b1 env s x1 v1,
+  (b1 -> env |-- ([x1], s) ---> ([encode v1], s)) ->
+  (b1 ->
+    env |-- ([If Less [Const 0; Const 1] x1 (Const 0)], s) ---> ([encode (value_otherwise v1)], s)).
+Proof.
+  intros.
+  apply H in X.
+  repeat econstructor; eauto.
+Qed.
+(* Hint Resolve auto_otherwise : automation. *)
+
+(* bool *)
+
+Theorem auto_bool_F : forall env s,
+  env |-- ([Const 0], s) ---> ([encode false], s).
+Proof.
+  intros. apply Eval_Const.
+Qed.
+Hint Resolve auto_bool_F : automation.
+
+Theorem auto_bool_T : forall env s,
+  env |-- ([Const 1], s) ---> ([encode true], s).
+Proof.
+  intros. apply Eval_Const.
+Qed.
+Hint Resolve auto_bool_T : automation.
+
 Theorem auto_bool_not : forall env s x1 b,
-  env |- ([x1], s) ---> ([refine b], s) ->
-  env |- ([Op Sub [Const 1; x1]], s) ---> ([refine (negb b)], s).
+  env |-- ([x1], s) ---> ([encode b], s) ->
+  env |-- ([Op Sub [Const 1; x1]], s) ---> ([encode (negb b)], s).
 Proof.
   intros env s x1 b H.
   Eval_eq.
@@ -118,97 +126,100 @@ Qed.
 Hint Resolve auto_bool_not : automation.
 
 Theorem auto_bool_and : forall env s x1 x2 bA bB,
-  env |- ([x1], s) ---> ([refine bA], s) ->
-  env |- ([x2], s) ---> ([refine bB], s) ->
-  env |- ([Op Sub [Op FunSyntax.Add [x1; x2]; Const 1]], s) ---> ([refine (andb bA bB)], s).
+  env |-- ([x1], s) ---> ([encode bA], s) ->
+  env |-- ([x2], s) ---> ([encode bB], s) ->
+  env |-- ([Op Sub [Op FunSyntax.Add [x1; x2]; Const 1]], s) ---> ([encode (andb bA bB)], s).
 Proof.
   intros env s x1 x2 bA bB H1 H2.
-  destruct (refine bA) eqn:HbA; destruct (refine bB) eqn:HbB; simpl in *.
-  all: unfold refine in *; simpl in *; destruct bA; destruct bB; inversion HbA; inversion HbB; subst.
+  destruct (encode bA) eqn:HbA; destruct (encode bB) eqn:HbB; simpl in *.
+  all: unfold encode in *; simpl in *; destruct bA; destruct bB; inversion HbA; inversion HbB; subst.
   all: Eval_eq.
 Qed.
 Hint Resolve auto_bool_and : automation.
 
 Theorem auto_bool_iff : forall env s x1 x2 bA bB,
-  env |- ([x1], s) ---> ([refine bA], s) ->
-  env |- ([x2], s) ---> ([refine bB], s) ->
-  env |- ([If Equal [x1; x2] (Const 1) (Const 0)], s) ---> ([refine (Bool.eqb bA bB)], s).
+  env |-- ([x1], s) ---> ([encode bA], s) ->
+  env |-- ([x2], s) ---> ([encode bB], s) ->
+  env |-- ([If Equal [x1; x2] (Const 1) (Const 0)], s) ---> ([encode (Bool.eqb bA bB)], s).
 Proof.
   intros env s x1 x2 bA bB H1 H2.
-  destruct (refine bA) eqn:HbA; destruct (refine bB) eqn:HbB; simpl in *.
-  all: unfold refine in *; simpl in *; destruct bA; destruct bB; inversion HbA; inversion HbB; subst.
+  destruct (encode bA) eqn:HbA; destruct (encode bB) eqn:HbB; simpl in *.
+  all: unfold encode in *; simpl in *; destruct bA; destruct bB; inversion HbA; inversion HbB; subst.
   all: Eval_eq.
 Qed.
 Hint Resolve auto_bool_iff : automation.
 
 Theorem last_bool_if : forall env s x_g x_t x_f (b : bool) t f,
-  env |- ([x_g], s) ---> ([refine b], s) ->
-  env |- ([x_t], s) ---> ([t], s) ->
-  env |- ([x_f], s) ---> ([f], s) ->
-  env |- ([If Equal [x_g; Const 1] x_t x_f], s) ---> ([if b then t else f], s).
+  env |-- ([x_g], s) ---> ([encode b], s) ->
+  env |-- ([x_t], s) ---> ([t], s) ->
+  env |-- ([x_f], s) ---> ([f], s) ->
+  env |-- ([If Equal [x_g; Const 1] x_t x_f], s) ---> ([if b then t else f], s).
 Proof.
   intros env s x_g x_t x_f b t f H1 H2 H3.
-  destruct (refine b) eqn:Hb; simpl in *.
-  all: unfold refine in *; simpl in *; destruct b; inversion Hb; subst.
+  destruct (encode b) eqn:Hb; simpl in *.
+  all: unfold encode in *; simpl in *; destruct b; inversion Hb; subst.
   all: Eval_eq.
 Qed.
 Hint Resolve last_bool_if : automation.
 
 (* num *)
 
-Theorem auto_num_const_zero : forall env s,
-  env |- ([Const 0], s) ---> ([Num 0], s).
+(* Theorem auto_num_const_zero : forall env s,
+  env |-- ([Const 0], s) ---> ([Num 0], s).
 Proof.
   intros. apply Eval_Const.
 Qed.
-Hint Resolve auto_num_const_zero : automation.
+Hint Resolve auto_num_const_zero : automation. *)
 
 Theorem auto_num_const : forall env s n,
-  env |- ([Const n], s) ---> ([Num n], s).
+  env |-- ([Const n], s) ---> ([Num n], s).
 Proof.
   intros. apply Eval_Const.
 Qed.
 Hint Resolve auto_num_const : automation.
 
 Theorem auto_num_add : forall b0 b1 env s0 s1 s2 x1 x2 n1 n2,
-  (b0 -> env |- ([x1], s0) ---> ([Num n1], s1)) ->
-  (b1 -> env |- ([x2], s1) ---> ([Num n2], s2)) ->
-  (b0 /\ b1 -> env |- ([Op FunSyntax.Add [x1; x2]], s0) ---> ([Num (n1 + n2)], s2)).
+  (b0 -> env |-- ([x1], s0) ---> ([encode n1], s1)) ->
+  (b1 -> env |-- ([x2], s1) ---> ([encode n2], s2)) ->
+  (b0 /\ b1 -> env |-- ([Op FunSyntax.Add [x1; x2]], s0) ---> ([encode (n1 + n2)], s2)).
 Proof.
   intros.
   destruct H1.
   repeat econstructor; eauto.
 Qed.
+Hint Resolve auto_num_add : automation.
 
 Theorem auto_num_sub : forall b0 b1 env s0 s1 s2 x1 x2 n1 n2,
-  (b0 -> env |- ([x1], s0) ---> ([Num n1], s1)) ->
-  (b1 -> env |- ([x2], s1) ---> ([Num n2], s2)) ->
-  (b0 /\ b1 -> env |- ([Op FunSyntax.Sub [x1; x2]], s0) ---> ([Num (n1 - n2)], s2)).
+  (b0 -> env |-- ([x1], s0) ---> ([encode n1], s1)) ->
+  (b1 -> env |-- ([x2], s1) ---> ([encode n2], s2)) ->
+  (b0 /\ b1 -> env |-- ([Op FunSyntax.Sub [x1; x2]], s0) ---> ([encode (n1 - n2)], s2)).
 Proof.
   intros.
   destruct H1.
   repeat econstructor; eauto.
 Qed.
+Hint Resolve auto_num_sub : automation.
 
 Theorem auto_num_div : forall b0 b1 env s0 s1 s2 x1 x2 n1 n2,
-  (b0 -> env |- ([x1], s0) ---> ([Num n1], s1)) ->
-  (b1 -> env |- ([x2], s1) ---> ([Num n2], s2)) ->
-  (b0 /\ b1 /\ n2 <> 0 -> env |- ([Op FunSyntax.Div [x1; x2]], s0) ---> ([Num (n1 / n2)], s2)).
+  (b0 -> env |-- ([x1], s0) ---> ([encode n1], s1)) ->
+  (b1 -> env |-- ([x2], s1) ---> ([encode n2], s2)) ->
+  (b0 /\ b1 /\ n2 <> 0 -> env |-- ([Op FunSyntax.Div [x1; x2]], s0) ---> ([encode (n1 / n2)], s2)).
 Proof.
   intros.
   destruct H1; destruct H2.
   repeat econstructor; eauto.
-  rewrite <- Nat.eqb_neq in *; simpl; rewrite H3; unfold return_; reflexivity.
+  rewrite <- Nat.eqb_neq in *; simpl; rewrite H3; reflexivity.
 Qed.
+Hint Resolve auto_num_div : automation.
 
 Theorem auto_num_if_eq : forall {A}
     b0 b1 b2 b3 env s x1 x2 y z n1 n2 t f (a : A -> Value),
-  (b0 -> env |- ([x1], s) ---> ([Num n1], s)) ->
-  (b1 -> env |- ([x2], s) ---> ([Num n2], s)) ->
-  (b2 -> env |- ([y], s) ---> ([a t], s)) ->
-  (b3 -> env |- ([z], s) ---> ([a f], s)) ->
+  (b0 -> env |-- ([x1], s) ---> ([encode n1], s)) ->
+  (b1 -> env |-- ([x2], s) ---> ([encode n2], s)) ->
+  (b2 -> env |-- ([y], s) ---> ([a t], s)) ->
+  (b3 -> env |-- ([z], s) ---> ([a f], s)) ->
   b0 /\ b1 /\ (if n1 =? n2 then b2 else b3) ->
-  env |- ([If Equal [x1; x2] y z], s) ---> ([a (if n1 =? n2 then t else f)], s).
+  env |-- ([If Equal [x1; x2] y z], s) ---> ([a (if n1 =? n2 then t else f)], s).
 Proof.
   intros.
   destruct H3 as [Hb0 [Hb1 HbCond]].
@@ -218,18 +229,19 @@ Proof.
   all: repeat econstructor; eauto.
   all: match goal with
   | [ |- take_branch _ _ _ = _ ] => unfold take_branch, return_; reflexivity
-  | [ |- (_ |- (_, _) ---> (_, _)) ] => rewrite Heq; assumption
+  | [ |- (_ |-- (_, _) ---> (_, _)) ] => rewrite Heq; assumption
   end.
 Qed.
+Hint Resolve auto_num_if_eq : automation.
 
 Theorem auto_num_if_less : forall {A}
     b0 b1 b2 b3 env s x1 x2 y z n1 n2 t f (a : A -> Value),
-  (b0 -> env |- ([x1], s) ---> ([Num n1], s)) ->
-  (b1 -> env |- ([x2], s) ---> ([Num n2], s)) ->
-  (b2 -> env |- ([y], s) ---> ([a t], s)) ->
-  (b3 -> env |- ([z], s) ---> ([a f], s)) ->
+  (b0 -> env |-- ([x1], s) ---> ([encode n1], s)) ->
+  (b1 -> env |-- ([x2], s) ---> ([encode n2], s)) ->
+  (b2 -> env |-- ([y], s) ---> ([a t], s)) ->
+  (b3 -> env |-- ([z], s) ---> ([a f], s)) ->
   b0 /\ b1 /\ (if n1 <? n2 then b2 else b3) ->
-  env |- ([If Less [x1; x2] y z], s) ---> ([a (if n1 <? n2 then t else f)], s).
+  env |-- ([If Less [x1; x2] y z], s) ---> ([a (if n1 <? n2 then t else f)], s).
 Proof.
   intros.
   destruct H3 as [Hb0 [Hb1 HbCond]].
@@ -239,23 +251,25 @@ Proof.
   all: repeat econstructor; eauto.
   all: match goal with
   | [ |- take_branch _ _ _ = _ ] => unfold take_branch, return_; reflexivity
-  | [ |- (_ |- (_, _) ---> (_, _)) ] => rewrite Heq; assumption
+  | [ |- (_ |-- (_, _) ---> (_, _)) ] => rewrite Heq; assumption
   end.
 Qed.
+Hint Resolve auto_num_if_less : automation.
 
 (* list *)
 
 Theorem auto_list_nil : forall env s,
-  env |- ([Const 0], s) ---> ([refine []], s).
+  env |-- ([Const 0], s) ---> ([encode []], s).
 Proof.
   intros; econstructor.
 Qed.
+Hint Resolve auto_list_nil : automation.
 
 Theorem auto_list_cons : forall {A} `{Refinable A} b0 b1 env s x1 x2 x xs,
-  (b0 -> env |- ([x1], s) ---> ([refine x], s)) ->
-  (b1 -> env |- ([x2], s) ---> ([refine xs], s)) ->
+  (b0 -> env |-- ([x1], s) ---> ([encode x], s)) ->
+  (b1 -> env |-- ([x2], s) ---> ([encode xs], s)) ->
   (b0 /\ b1 ->
-    env |- ([Op Cons [x1; x2]], s) ---> ([refine (x :: xs)], s)).
+    env |-- ([Op Cons [x1; x2]], s) ---> ([encode (x :: xs)], s)).
 Proof.
   intros.
   match goal with
@@ -264,22 +278,23 @@ Proof.
   end.
   repeat econstructor; eauto.
 Qed.
+Hint Resolve auto_list_cons : automation.
 
-(* TODO(kπ) check this. *)
 Theorem auto_list_case : forall {A B} `{ra : Refinable A} `{rb : Refinable B}
     b0 b1 b2 env s x0 x1 x2 n1 n2 (v0 : list A) v1 v2,
-  (b0 -> env |- ([x0], s) ---> ([refine v0], s)) ->
-  (b1 -> env |- ([x1], s) ---> ([rb.(refine) v1], s)) ->
+  (b0 -> env |-- ([x0], s) ---> ([encode v0], s)) ->
+  (b1 -> env |-- ([x1], s) ---> ([rb.(encode) v1], s)) ->
   (forall y1 y2,
       b2 y1 y2 ->
-      (Env.insert (value_name n2, Some (refine y2))
-        (Env.insert (value_name n1, Some (ra.(refine) y1)) env)) |- ([x2], s) ---> ([rb.(refine) (v2 y1 y2)], s)) ->
-  NoDup ([value_name n1] ++ free_vars x0) ->
+      (Env.insert (name_enc n2, Some (encode y2))
+        (Env.insert (name_enc n1, Some (ra.(encode) y1)) env)) |-- ([x2], s) --->
+      ([rb.(encode) (v2 y1 y2)], s)) ->
+  NoDup ([name_enc n1] ++ free_vars x0) ->
   b0 /\ (v0 = [] -> b1) /\ (forall y1 y2, v0 = y1 :: y2 -> b2 y1 y2) ->
-  env |- ([If Equal [x0; Const 0] x1
-            (Let (value_name n1) (Op Head [x0])
-              (Let (value_name n2) (Op Tail [x0]) x2))], s) --->
-         ([rb.(refine) (list_CASE v0 v1 v2)], s).
+  env |-- ([If Equal [x0; Const 0] x1
+            (Let (name_enc n1) (Op Head [x0])
+              (Let (name_enc n2) (Op Tail [x0]) x2))], s) --->
+         ([rb.(encode) (list_CASE v0 v1 v2)], s).
 Proof.
   intros.
   destruct H3 as [Hb0 [Hb1 Hb2]].
@@ -291,21 +306,23 @@ Proof.
     rewrite NoDup_cons_iff in *; destruct H2.
     Eval_eq.
     + rewrite remove_env_update; eauto.
-    + simpl; unfold return_; reflexivity.
+    + simpl; reflexivity.
 Qed.
+Hint Resolve auto_list_case : automation.
 
 (* option *)
 
 Theorem auto_option_none : forall {A} `{Refinable A} env s,
-  env |- ([Const 0], s) ---> ([refine None], s).
+  env |-- ([Const 0], s) ---> ([encode None], s).
 Proof.
   intros; econstructor.
 Qed.
+Hint Resolve auto_option_none : automation.
 
 Theorem auto_option_some : forall {A} `{Refinable A} b0 env s x1 x,
-  (b0 -> env |- ([x1], s) ---> ([refine x], s)) ->
+  (b0 -> env |-- ([x1], s) ---> ([encode x], s)) ->
   (b0 ->
-    env |- ([Op Cons [x1; Const 0]], s) ---> ([refine (Some x)], s)).
+    env |-- ([Op Cons [x1; Const 0]], s) ---> ([encode (Some x)], s)).
 Proof.
   intros.
   match goal with
@@ -314,16 +331,17 @@ Proof.
   end.
   repeat econstructor; eauto.
 Qed.
+Hint Resolve auto_option_some : automation.
 
 Theorem auto_option_case : forall {A B} `{Refinable A} `{rb : Refinable B} (v0 : option A) b0 b1 b2 env s x0 x1 x2 n v1 v2,
-  (b0 -> env |- ([x0],s) ---> ([refine v0],s)) ->
-  (b1 -> env |- ([x1],s) ---> ([rb.(refine) v1],s)) ->
+  (b0 -> env |-- ([x0],s) ---> ([encode v0],s)) ->
+  (b1 -> env |-- ([x1],s) ---> ([rb.(encode) v1],s)) ->
   (forall y1, b2 y1 ->
-    (Env.insert (value_name n, Some (refine y1)) env) |- ([x2],s) ---> ([rb.(refine) (v2 y1)],s)) ->
+    (Env.insert (name_enc n, Some (encode y1)) env) |-- ([x2],s) ---> ([rb.(encode) (v2 y1)],s)) ->
   b0 /\ (v0 = None -> b1) /\ (forall y1, v0 = Some y1 -> b2 y1) ->
-  env |- ([If Equal [x0; Const 0] x1
-            (Let (value_name n) (Op Head [x0]) x2)], s) --->
-         ([rb.(refine) (option_CASE v0 v1 v2)], s).
+  env |-- ([If Equal [x0; Const 0] x1
+            (Let (name_enc n) (Op Head [x0]) x2)], s) --->
+         ([rb.(encode) (option_CASE v0 v1 v2)], s).
 Proof.
   intros.
   destruct H3 as [Hb0 [Hb1 Hb2]].
@@ -334,12 +352,13 @@ Proof.
   - apply H1 in Hb1; try reflexivity.
     Eval_eq.
 Qed.
+Hint Resolve auto_option_case : automation.
 
 (* pair *)
 
 Theorem auto_pair_fst : forall {A B} `{Refinable A} `{Refinable B} b0 env s x1 (x : A * B),
-  (b0 -> env |- ([x1], s) ---> ([refine x], s)) ->
-  (b0 -> env |- ([Op Head [x1]], s) ---> ([refine (fst x)], s)).
+  (b0 -> env |-- ([x1], s) ---> ([encode x], s)) ->
+  (b0 -> env |-- ([Op Head [x1]], s) ---> ([encode (fst x)], s)).
 Proof.
   intros.
   match goal with
@@ -349,10 +368,11 @@ Proof.
   destruct x; simpl in *.
   repeat econstructor; eauto.
 Qed.
+Hint Resolve auto_pair_fst : automation.
 
 Theorem auto_pair_snd : forall {A B} `{Refinable A} `{Refinable B} b0 env s x1 (x : A * B),
-  (b0 -> env |- ([x1], s) ---> ([refine x], s)) ->
-  (b0 -> env |- ([Op Tail [x1]], s) ---> ([refine (snd x)], s)).
+  (b0 -> env |-- ([x1], s) ---> ([encode x], s)) ->
+  (b0 -> env |-- ([Op Tail [x1]], s) ---> ([encode (snd x)], s)).
 Proof.
   intros.
   match goal with
@@ -362,12 +382,13 @@ Proof.
   destruct x; simpl in *.
   repeat econstructor; eauto.
 Qed.
+Hint Resolve auto_pair_fst : automation.
 
 Theorem auto_pair_cons : forall {A B} `{Refinable A} `{Refinable B} b0 b1 env s x1 x2 (x : A) (y : B),
-  (b0 -> env |- ([x1], s) ---> ([refine x], s)) ->
-  (b1 -> env |- ([x2], s) ---> ([refine y], s)) ->
+  (b0 -> env |-- ([x1], s) ---> ([encode x], s)) ->
+  (b1 -> env |-- ([x2], s) ---> ([encode y], s)) ->
   (b0 /\ b1 ->
-    env |- ([Op Cons [x1; x2]], s) ---> ([refine (x, y)], s)).
+    env |-- ([Op Cons [x1; x2]], s) ---> ([encode (x, y)], s)).
 Proof.
   intros.
   match goal with
@@ -376,20 +397,21 @@ Proof.
   end.
   repeat econstructor; eauto.
 Qed.
+Hint Resolve auto_pair_cons : automation.
 
 Theorem auto_pair_case : forall {A1 A2 B} `{ra1 : Refinable A1} `{ra2 : Refinable A2} `{rb : Refinable B}
     b0 b1 env s x0 x1 n1 n2 (v0 : A1 * A2) v1,
-  (b0 -> env |- ([x0], s) ---> ([refine v0], s)) ->
+  (b0 -> env |-- ([x0], s) ---> ([encode v0], s)) ->
   (forall y1 y2,
       b1 y1 y2 ->
-      (Env.insert (value_name n2, Some (ra2.(refine) y2))
-        (Env.insert (value_name n1, Some (ra1.(refine) y1)) env)) |- ([x1], s) --->
-      ([rb.(refine) (v1 y1 y2)], s)) ->
-  NoDup ([value_name n1] ++ [value_name n2] ++ free_vars x0) ->
+      (Env.insert (name_enc n2, Some (ra2.(encode) y2))
+        (Env.insert (name_enc n1, Some (ra1.(encode) y1)) env)) |-- ([x1], s) --->
+      ([rb.(encode) (v1 y1 y2)], s)) ->
+  NoDup ([name_enc n1] ++ [name_enc n2] ++ free_vars x0) ->
   b0 /\ (forall y1 y2, v0 = (y1, y2) -> b1 y1 y2) ->
-  env |- ([Let (value_name n1) (Op Head [x0])
-            (Let (value_name n2) (Op Tail [x0]) x1)], s) --->
-  ([rb.(refine) (pair_CASE v0 v1)], s).
+  env |-- ([Let (name_enc n1) (Op Head [x0])
+            (Let (name_enc n2) (Op Tail [x0]) x1)], s) --->
+  ([rb.(encode) (pair_CASE v0 v1)], s).
 Proof.
   intros.
   destruct H2 as [Hb0 Hb1].
@@ -401,8 +423,296 @@ Proof.
     repeat rewrite NoDup_cons_iff in *; destruct H1; destruct H2.
     rewrite not_in_cons in *; destruct H1.
     rewrite remove_env_update; eauto.
-  - simpl; unfold return_; reflexivity.
+  - simpl; reflexivity.
 Qed.
+Hint Resolve auto_pair_case : automation.
+
+(* Was only needed in th eoriginal implementation, because parsing goes through Values *)
+(* Maybe we'll need it now *)
+(*
+(* deep *)
+
+Fixpoint deep (v : Value) : Value :=
+  match v with
+  | Num n => value_cons (encode true) (encode n)
+  | Pair x y => value_cons (encode false) (value_cons (deep x) (deep y))
+  end.
+
+Theorem auto_v_Num : forall b0 env s x1 n,
+  (b0 -> env |-- ([x1], s) ---> ([Num n], s)) ->
+  b0 ->
+  env |-- ([Op Cons [Const 1; x1]], s) ---> ([deep (Num n)], s).
+Proof.
+  intros b0 env s x1 n H H0.
+  apply H in H0.
+  simpl.
+  repeat econstructor; eauto.
+Qed.
+Hint Resolve auto_v_Num : automation.
+
+Theorem auto_v_Pair : forall b0 b1 env s x1 x2 x y,
+  (b0 -> env |-- ([x1], s) ---> ([deep x], s)) ->
+  (b1 -> env |-- ([x2], s) ---> ([deep y], s)) ->
+  b0 /\ b1 ->
+  env |-- ([Op Cons [Const 0; Op Cons [x1; x2]]], s) ---> ([deep (Pair x y)], s).
+Proof.
+  intros b0 b1 env s x1 x2 x y H1 H2 [Hb0 Hb1].
+  apply H1 in Hb0.
+  apply H2 in Hb1.
+  simpl.
+  repeat econstructor; eauto.
+Qed.
+Hint Resolve auto_v_Pair : automation.
+
+Theorem auto_v_isNum : forall b0 env s x1 x,
+  (b0 -> env |-- ([x1], s) ---> ([deep x], s)) ->
+  b0 ->
+  env |-- ([Op Head [x1]], s) ---> ([encode (value_isNum x)], s).
+Proof.
+  intros b0 env s x1 x H H0.
+  apply H in H0.
+  destruct x; simpl; repeat econstructor; eauto.
+Qed.
+Hint Resolve auto_v_isNum : automation.
+
+Theorem auto_v_getNum : forall b0 env s x1 x,
+  (b0 -> env |-- ([x1], s) ---> ([deep x], s)) ->
+  b0 ->
+  env |-- ([If Equal [Op Head [x1]; Const 0] (Const 0) (Op Tail [x1])], s) --->
+  ([Num (value_getNum x)], s).
+Proof.
+  intros b0 env s x1 x H H0.
+  apply H in H0.
+  destruct x; simpl; repeat econstructor; Eval_eq.
+Qed.
+Hint Resolve auto_v_getNum : automation.
+
+Theorem auto_v_head : forall b0 env s x1 x,
+  lookup_fun (name_enc_str "h"%string) s.(funs) =
+    Some ([name_enc_str "x"%string],
+          If Equal [Op Head [Var (name_enc_str "x"%string)]; Const 1]
+            (Var (name_enc_str "x"%string)) (Op Head [Op Tail [Var (name_enc_str "x"%string)]])) ->
+  (b0 -> env |-- ([x1], s) ---> ([deep x], s)) ->
+  b0 ->
+  env |-- ([Call (name_enc_str "h"%string) [x1]], s) ---> ([deep (value_head x)], s).
+Proof.
+  intros b0 env s x1 x Hlookup H H0.
+  destruct x; simpl.
+  all: eapply Eval_Call_thm.
+  all: try match goal with
+  | [ |- ?env |-- ([?x1], ?s) ---> (_, _) ] => eauto
+  end.
+  all: econstructor; unfold env_and_body; simpl in *.
+  all: destruct (lookup_fun (name_enc_str "h") (funs s)) eqn:?; try destruct p.
+  all: try inversion Hlookup; clear Hlookup; subst; simpl.
+  all: f_equal; f_equal.
+  all: Eval_eq.
+  all: try rewrite Env.lookup_insert_eq; try reflexivity.
+  all: simpl; unfold return_; try reflexivity.
+  all: Eval_eq.
+  all: try rewrite Env.lookup_insert_eq; try reflexivity.
+Qed.
+Hint Resolve auto_v_head : automation.
+
+Theorem auto_v_tail : forall b0 env s x1 x,
+  lookup_fun (name_enc_str "t") s.(funs) =
+    Some ([name_enc_str "x"],
+          If Equal [Op Head [Var (name_enc_str "x")]; Const 1]
+            (Var (name_enc_str "x")) (Op Tail [Op Tail [Var (name_enc_str "x")]])) ->
+  (b0 -> env |-- ([x1], s) ---> ([deep x], s)) ->
+  b0 ->
+  env |-- ([Call (name_enc_str "t") [x1]], s) ---> ([deep (value_tail x)], s).
+Proof.
+  intros b0 env s x1 x Hlookup H H0.
+  destruct x; simpl.
+  all: eapply Eval_Call_thm.
+  all: try match goal with
+  | [ |- ?env |-- ([?x1], ?s) ---> (_, _) ] => eauto
+  end.
+  all: econstructor; unfold env_and_body; simpl in *.
+  all: destruct (lookup_fun (name_enc_str "t") (funs s)) eqn:?; try destruct p.
+  all: try inversion Hlookup; clear Hlookup; subst; simpl.
+  all: f_equal; f_equal.
+  all: Eval_eq.
+  all: try rewrite Env.lookup_insert_eq; try reflexivity.
+  all: simpl; unfold return_; try reflexivity.
+  all: Eval_eq.
+  all: try rewrite Env.lookup_insert_eq; try reflexivity.
+Qed.
+Hint Resolve auto_v_tail : automation.
+*)
+
+(* char *)
+
+Theorem auto_char_CHR : forall b0 env s x1 x,
+  (b0 -> env |-- ([x1], s) ---> ([Num x], s)) ->
+  b0 /\ x < 256 ->
+  env |-- ([x1], s) ---> ([encode (ascii_of_nat x)], s).
+Proof.
+  intros b0 env s x1 x H H0.
+  destruct H0 as [Hb0 Hx].
+  simpl.
+  rewrite nat_ascii_embedding; auto.
+Qed.
+Hint Resolve auto_char_CHR : automation.
+
+Theorem auto_char_ORD : forall b0 env s x1 x,
+  (b0 -> env |-- ([x1], s) ---> ([encode x], s)) ->
+  b0 ->
+  env |-- ([x1], s) ---> ([Num (nat_of_ascii x)], s).
+Proof.
+  intros b0 env s x1 x H H0.
+  apply H in H0.
+  simpl in *.
+  assumption.
+Qed.
+Hint Resolve auto_char_ORD : automation.
+
+(* word *)
+
+Definition value_word {n} (w : word n) : Value :=
+  Num (Z.to_nat (word.unsigned w)).
+
+Theorem auto_word4_n2w : forall b0 env s x1 x,
+  (b0 -> env |-- ([x1], s) ---> ([Num x], s)) ->
+  b0 /\ x < 16 ->
+  env |-- ([x1], s) ---> ([value_word ((word.of_Z (Z.of_nat x)) : word4)], s).
+Proof.
+  intros b0 env s x1 x H H0.
+  destruct H0 as [Hb0 Hx].
+  apply H in Hb0.
+  unfold value_word.
+  rewrite word.unsigned_of_Z.
+  unfold word.wrap.
+  cbn.
+  assert ((Z.to_nat (Z.of_nat x mod 16)) = x).
+  2: { rewrite H0. eapply Hb0. }
+  rewrite Z.mod_small; lia.
+Qed.
+Hint Resolve auto_word4_n2w : automation.
+
+Theorem auto_word64_n2w : forall b0 env s x1 x,
+  (b0 -> env |-- ([x1], s) ---> ([Num x], s)) ->
+  b0 /\ x < 2 ^ 64 ->
+  env |-- ([x1], s) ---> ([value_word ((word.of_Z (Z.of_nat x)) : word64)], s).
+Proof.
+  intros b0 env s x1 x H H0.
+  destruct H0 as [Hb0 Hx].
+  apply H in Hb0.
+  unfold value_word.
+  rewrite word.unsigned_of_Z.
+  unfold word.wrap.
+  cbn.
+  assert ((Z.to_nat (Z.of_nat x mod (2 ^ 64))) = x).
+  2: { cbn in H0. rewrite H0. eapply Hb0. }
+  rewrite Z.mod_small; try lia.
+  apply inj_lt in Hx.
+  split; try lia.
+  rewrite inj_pow in Hx.
+  simpl  Z.of_nat in Hx.
+  assumption.
+Qed.
+Hint Resolve auto_word64_n2w : automation.
+
+Theorem auto_word4_w2n : forall b0 env s x1 x,
+  (b0 -> env |-- ([x1], s) ---> ([value_word (x : word4)], s)) ->
+  b0 ->
+  env |-- ([x1], s) ---> ([Num (Z.to_nat (word.unsigned x))], s).
+Proof.
+  intros b0 env s x1 x H Hb0.
+  apply H in Hb0.
+  unfold value_word in *.
+  assumption.
+Qed.
+Hint Resolve auto_word4_w2n : automation.
+
+Theorem auto_word64_w2n : forall b0 env s x1 x,
+  (b0 -> env |-- ([x1], s) ---> ([value_word (x : word64)], s)) ->
+  b0 ->
+  env |-- ([x1], s) ---> ([Num (Z.to_nat (word.unsigned x))], s).
+Proof.
+  intros b0 env s x1 x H Hb0.
+  apply H in Hb0.
+  unfold value_word in *.
+  assumption.
+Qed.
+Hint Resolve auto_word64_w2n : automation.
+
+(* TODO(kπ) Skipped common definitions and some automation for cons and case *)
+
+(* TODO(kπ) Token *)
+
+(* cmp *)
+
+Global Instance Refinable_cmp : Refinable ImpSyntax.cmp :=
+{ encode cmp :=
+  match cmp with
+  | ImpSyntax.Equal => value_name "Equal"
+  | ImpSyntax.Less => value_name "Less"
+  end }.
+
+(* TODO(kπ) lammas *)
+
+(* exp *)
+
+Fixpoint encode_exp (e : ImpSyntax.exp) : Value :=
+  match e with
+  | ImpSyntax.Var n => value_list_of_values [value_name "Var"; Num n]
+  | ImpSyntax.Const n => value_list_of_values [value_name "Const"; value_word n]
+  | ImpSyntax.Add e1 e2 =>
+      value_list_of_values [value_name "Add"; encode_exp e1; encode_exp e2]
+  | ImpSyntax.Sub e1 e2 =>
+      value_list_of_values [value_name "Sub"; encode_exp e1; encode_exp e2]
+  | ImpSyntax.Div e1 e2 =>
+      value_list_of_values [value_name "Div"; encode_exp e1; encode_exp e2]
+  | ImpSyntax.Read e1 e2 =>
+      value_list_of_values [value_name "Read"; encode_exp e1; encode_exp e2]
+  end.
+
+Global Instance Refinable_exp : Refinable ImpSyntax.exp :=
+ { encode := encode_exp }.
+
+(* TODO(kπ) lammas *)
+
+(* test *)
+
+Fixpoint encode_test (test : ImpSyntax.test) : Value :=
+  match test with
+  | ImpSyntax.Test c e1 e2 =>
+      value_list_of_values [value_name "Test"; encode c; encode_exp e1; encode_exp e2]
+  | ImpSyntax.And t1 t2 =>
+      value_list_of_values [value_name "And"; encode_test t1; encode_test t2]
+  | ImpSyntax.Or t1 t2 =>
+      value_list_of_values [value_name "Or"; encode_test t1; encode_test t2]
+  | ImpSyntax.Not t =>
+      value_list_of_values [value_name "Not"; encode_test t]
+  end.
+
+Global Instance Refinable_test : Refinable ImpSyntax.test :=
+{ encode := encode_test }.
+
+(* TODO(kπ) lammas *)
+
+(* list *)
+
+(* TODO(kπ) lammas *)
+
+(* app_list *)
+
+Fixpoint encode_app_list {A} `{Refinable A} (l : app_list A) : Value :=
+  match l with
+  | List xs =>
+      value_list_of_values [value_name "List"; encode xs]
+  | Append xs ys =>
+      value_list_of_values [value_name "Append"; encode_app_list xs;
+                            encode_app_list ys]
+  end.
+
+Global Instance Refinable_app_list {A} `{Refinable A} : Refinable (app_list A) :=
+{ encode := encode_app_list }.
+
+(* TODO(kπ) lammas *)
 
 (* TODO(kπ) continue *)
+
 
