coq/theories/functional/FunSemantics.v
@@ -36,6 +36,7 @@ Definition set_output (s : state) (out : list ascii) : state :=
 
 Definition return_ {A} (v : A) (s : state) : result A * state :=
   (Res v, s).
+Arguments return_ !_ !_ /.
 
 Definition fail {A} (s : state) : result A * state :=
   (Err Crash, s).
@@ -71,6 +72,7 @@ Definition take_branch (test : FunSyntax.test) (vs : list Value) (s : state) : r
   | FunSyntax.Less, [Num m; Num n] => return_ (m <? n) s
   | _, _ => fail s
   end.
+Arguments take_branch !_ !_ !_ /.
 
 Fixpoint make_env (keys : list name) (values : list Value) (acc : Env.env) : Env.env :=
   match keys, values with
@@ -84,68 +86,71 @@ Fixpoint lookup_fun (n : name) (fs : list FunSyntax.dec) : option (list name * F
   | [] => None
   | FunSyntax.Defun k ps body :: rest => if k =? n then Some (ps, body) else lookup_fun n rest
   end.
+Arguments lookup_fun !_ !_ /.
 
 Definition env_and_body (n : name) (args : list Value) (s : state) : option (Env.env * FunSyntax.exp) :=
   match lookup_fun n s.(funs) with
   | None => None
   | Some (params, body) => if List.length params =? List.length args then Some (make_env params args Env.empty, body) else None
   end.
+Arguments env_and_body !_ !_ /.
 
 Definition init_state (inp : llist ascii) (funs : list FunSyntax.dec) : state :=
   {| funs := funs; clock := 0; input := inp; output := [] |}.
 
-Reserved Notation "env '|-' ( es , s1 ) '--->' ( vs , s2 )" (at level 40, es at next level, vs at next level).
+Reserved Notation "env '|--' ( es , s1 ) '--->' ( vs , s2 )" (at level 40, es at next level, vs at next level).
 
-(* TODO(ask Magnus) why he likes using `list of exp`, instead of exp *)
+(* Ask Magnus why he likes using `list of exp`, instead of exp *)
+(* Answer: to avoid mutual recursion *)
 Inductive eval : Env.env -> list FunSyntax.exp -> state -> list Value -> state -> Prop :=
 | Eval_Nil : forall env s,
-  env |- ([], s) ---> ([], s)
+  env |-- ([], s) ---> ([], s)
 | Eval_Cons : forall env exp1 v exp2 exps vs s1 s2 s3,
   forall
-    (EVAL_HEAD : env |- ([exp1],  s1) ---> ([v],  s2))
-    (EVAL_TAIL : env |- ((exp2 :: exps),  s2) ---> (vs,  s3)),
-  env |- ((exp1 :: exp2 :: exps),  s1) ---> ((v :: vs),  s3)
+    (EVAL_HEAD : env |-- ([exp1],  s1) ---> ([v],  s2))
+    (EVAL_TAIL : env |-- ((exp2 :: exps),  s2) ---> (vs,  s3)),
+  env |-- ((exp1 :: exp2 :: exps),  s1) ---> ((v :: vs),  s3)
 | Eval_Const : forall env n s,
-  env |- ([FunSyntax.Const n],  s) ---> ([Num n],  s)
+  env |-- ([FunSyntax.Const n],  s) ---> ([Num n],  s)
 | Eval_Var : forall env n v s,
   forall
   (ENV_LOOKUP : Env.lookup env n = Some v),
-  env |- ([FunSyntax.Var n],  s) ---> ([v],  s)
+  env |-- ([FunSyntax.Var n],  s) ---> ([v],  s)
 | Eval_Op : forall env exps s1 vs s2 op v s3,
   forall
-    (EVAL_ARGS : env |- (exps,  s1) ---> (vs,  s2))
+    (EVAL_ARGS : env |-- (exps,  s1) ---> (vs,  s2))
     (EVAL_OP : eval_op op vs s2 = (Res v, s3)),
-  env |- ([FunSyntax.Op op exps],  s1) ---> ([v],  s3)
+  env |-- ([FunSyntax.Op op exps],  s1) ---> ([v],  s3)
 | Eval_Let : forall env exp1 exp2 s1 v1 s2 n s3 v2,
   forall
-    (EVAL_RHS : env |- ([exp1],  s1) ---> ([v1],  s2))
-    (EVAL_RES : (Env.insert (n, Some v1) env) |- ([exp2],  s2) ---> ([v2],  s3)),
-  env |- ([FunSyntax.Let n exp1 exp2],  s1) ---> ([v2],  s3)
+    (EVAL_RHS : env |-- ([exp1],  s1) ---> ([v1],  s2))
+    (EVAL_RES : (Env.insert (n, Some v1) env) |-- ([exp2],  s2) ---> ([v2],  s3)),
+  env |-- ([FunSyntax.Let n exp1 exp2],  s1) ---> ([v2],  s3)
 | Eval_If : forall env exps s1 vs s2 test b expt expf v s3,
   forall
-    (EVAL_COND : env |- (exps,  s1) ---> (vs,  s2))
+    (EVAL_COND : env |-- (exps,  s1) ---> (vs,  s2))
     (TAKE_BRANCH : take_branch test vs s2 = (Res b, s2))
-    (EVAL_RES : env |- ([if b then expt else expf],  s2) ---> ([v],  s3)),
-  env |- ([FunSyntax.If test exps expt expf],  s1) ---> ([v],  s3)
+    (EVAL_RES : env |-- ([if b then expt else expf],  s2) ---> ([v],  s3)),
+  env |-- ([FunSyntax.If test exps expt expf],  s1) ---> ([v],  s3)
 | Eval_Call : forall env exps s1 vs s2 fname v s3 new_env body,
   forall
-    (EVAL_ARGS : env |- (exps,  s1) ---> (vs,  s2))
+    (EVAL_ARGS : env |-- (exps,  s1) ---> (vs,  s2))
     (ENV_BODY : env_and_body fname vs s2 = Some (new_env, body))
-    (EVAL_BODY : new_env |- ([body],  s2) ---> ([v],  s3)),
-  env |- ([FunSyntax.Call fname exps],  s1) ---> ([v],  s3)
-where "env '|-' ( es , s1 ) '--->' ( vs , s2 )" := (eval env es s1 vs s2).
+    (EVAL_BODY : new_env |-- ([body],  s2) ---> ([v],  s3)),
+  env |-- ([FunSyntax.Call fname exps],  s1) ---> ([v],  s3)
+where "env '|--' ( es , s1 ) '--->' ( vs , s2 )" := (eval env es s1 vs s2).
 
 Inductive eval_app : name -> list Value -> state -> (Value * state) -> Prop :=
 | App_intro : forall fname vs s1 v s2 new_env body,
   env_and_body fname vs s1 = Some (new_env, body) ->
-  new_env |- ([body], s1) ---> ([v], s2) ->
+  new_env |-- ([body], s1) ---> ([v], s2) ->
   eval_app fname vs s1 (v, s2).
 
 Theorem Eval_Call_thm :
   forall env exps s1 vs s2 fname v s3,
-  env |- (exps, s1) ---> (vs, s2) ->
+  env |-- (exps, s1) ---> (vs, s2) ->
   eval_app fname vs s2 (v, s3) ->
-  env |- ([FunSyntax.Call fname exps], s1) ---> ([v], s3).
+  env |-- ([FunSyntax.Call fname exps], s1) ---> ([v], s3).
 Proof.
   intros env exps s1 vs s2 fname v s3 H_eval_args H_app.
   inversion H_app; subst.
@@ -154,5 +159,5 @@ Qed.
 
 Definition prog_terminates (input : llist ascii) (p : FunSyntax.prog) (out : list ascii) : Prop :=
   exists s r,
-    Env.empty |- ([get_main p],  (init_state input (get_defs p))) ---> (r,  s) /\
+    Env.empty |-- ([get_main p],  (init_state input (get_defs p))) ---> (r,  s) /\
         out = s.(output).
