coq/theories/automation/Automation.v
@@ -1,9 +1,13 @@
 From impboot Require Import utils.Core.
+From coqutil Require Import dlet.
 Require Import impboot.functional.FunValues.
 Require Import impboot.functional.FunSyntax.
 Require Import impboot.functional.FunSemantics.
 Require Import impboot.automation.AutomationLemmas.
 Require Import impboot.utils.Llist.
+From Ltac2 Require Import Ltac2.
+From Ltac2 Require Import Message.
+Require Import Coq.derive.Derive.
 
 Ltac rewrite_let := match goal with
 | [ |- context C [?subterm] ] =>
@@ -18,26 +22,219 @@ Definition empty_state : state := init_state lnil [].
 
 (* TODO(kπ) figure out a good example, this one gets constant folded *)
 (* Example arith_example : forall n m,
-  exists prog, Env.empty |- (prog, empty_state) ---> ([Num (let x := 1 in x + n - m)], empty_state).
+  exists prog, Env.empty |-- (prog, empty_state) ---> ([Num (let x := 1 in x + n - m)], empty_state).
 Proof.
   intros.
   rewrite_let.
   eexists. (* TODO(kπ) this simplifies my function :/ Is this a problem with normal code?*)
   eapply auto_let; eauto; intros.
   repeat match goal with
-  | |- context[_ + _] => eapply auto_num_add; eauto
-  | |- context[_ - _] => eapply auto_num_sub; eauto
+  | |-- context[_ + _] => eapply auto_num_add; eauto
+  | |-- context[_ - _] => eapply auto_num_sub; eauto
   end.
   (* TODO(kπ) *)
 Qed. *)
 
-(*
-TODO(kπ) Problems:
-- in HOL4 (let x = a in b) is encoded as ((fn x => b) a) Do we have to do the
-  same? Add a preprocessing step or sth?
-- in the HOL4 version (AFAIK) only limited matches on datatypes are supported,
-  but the problem is that matches in HOL4 are represented using `CASE functions`
-  e.g.
-  list case [ ] f1 f2 = f1
-  list case (x :: xs) f1 f2 = f2 x xs
-*)
+(* Ltac2 compile (c : constr) := 1. *)
+
+(* Rupicola approach *)
+
+(* Ltac autostep :=
+  (* eapply trans_app ||
+  eapply trans_Var ||
+  eapply trans_Call ||
+  eapply trans_nil ||
+  eapply trans_cons || *)
+  (* eapply auto_otherwise || *)
+  eapply auto_bool_F ||
+  eapply auto_bool_T ||
+  eapply auto_bool_not ||
+  eapply auto_bool_and ||
+  eapply auto_bool_iff ||
+  eapply last_bool_if ||
+  (* eapply auto_num_const_zero || *)
+  eapply auto_num_const ||
+  eapply auto_num_add ||
+  eapply auto_num_sub ||
+  eapply auto_num_div ||
+  eapply auto_num_if_eq ||
+  eapply auto_num_if_less ||
+  eapply auto_list_nil ||
+  eapply auto_list_cons ||
+  eapply auto_list_case ||
+  eapply auto_option_none ||
+  eapply auto_option_some ||
+  eapply auto_option_case ||
+  eapply auto_pair_fst ||
+  eapply auto_pair_snd ||
+  eapply auto_pair_cons ||
+  eapply auto_pair_case ||
+  eapply auto_char_CHR ||
+  eapply auto_char_ORD ||
+  eapply auto_word4_n2w ||
+  eapply auto_word64_n2w ||
+  eapply auto_word4_w2n ||
+  eapply auto_word64_w2n ||
+  (* This gets applied to eagerly *)
+  eapply auto_let. *)
+
+(* Derive f1 SuchThat
+  (forall n m,
+    exists prog,
+      Env.empty |-- (prog, empty_state) --->
+      ([encode (letd x := 1 in x + n - m)], empty_state))
+  As f1_rpoof. *)
+
+Ltac2 Type rec clist := [
+  | Lnil
+  | Lcons (constr, clist)
+].
+
+Ltac2 compile (e : constr) (env : clist) : constr :=
+  match! e with
+  | _ |-- (_, _) ---> ([encode (dlet ?val ?body)], _) =>
+    open_constr:(auto_let
+    (* b1 *) _
+    (* b2 *) _
+    (* env *) _
+    (* x1 y1 *) _ _
+    (* s1 s2 s3 *) _ _ _
+    (* v1 *) ltac2:(val)
+    (* let_n *) _
+    (* f *) ltac2:(body)
+    (* eval v1 *) _
+    (* eval v2 *) _
+    (* b1 /\ b2 *) _
+    )
+  | _ |-- (_, _) ---> ([encode true], _) =>
+    open_constr:(auto_bool_T
+    (* env *) _
+    (* s *) _
+    )
+  | _ |-- (_, _) ---> ([encode false], _) =>
+    open_constr:(auto_bool_F
+    (* env *) _
+    (* s *) _
+    )
+  | _ |-- (_, _) ---> ([encode (negb _)], _) =>
+    open_constr:(auto_bool_not
+    (* env *) _
+    (* s *) _
+    (* x1 *) _
+    (* b *) _
+    (* eval x1 *) _
+    )
+  | _ |-- (_, _) ---> ([encode (andb _ _)], _) =>
+    open_constr:(auto_bool_and
+    (* env *) _
+    (* s *) _
+    (* x1 x2 *) _ _
+    (* bA bB *) _ _
+    (* eval x1 *) _
+    (* eval x2 *) _
+    )
+  | _ |-- (_, _) ---> ([encode (eqb _ _)], _) =>
+    open_constr:(auto_bool_iff
+    (* env *) _
+    (* s *) _
+    (* x1 x2 *) _ _
+    (* bA bB *) _ _
+    (* eval x1 *) _
+    (* eval x2 *) _
+    )
+  | _ |-- (_, _) ---> ([encode (if _ then _ else _)], _) =>
+    open_constr:(last_bool_if
+    (* env *) _
+    (* s *) _
+    (* x_g x_t x_f *) _ _ _
+    (* b t f *) _ _ _
+    (* eval x_g *) _
+    (* eval x_t *) _
+    (* eval x_f *) _
+    )
+  | _ |-- (_, _) ---> ([encode (_ + _)], _) =>
+    open_constr:(auto_num_add
+    (* b0 b1 *) _ _
+    (* env *) _
+    (* s0 s1 s2 *) _ _ _
+    (* x1 x2 *) _ _
+    (* n1 n2 *) _ _
+    (* eval x1 *) _
+    (* eval x2 *) _
+    (* b0 /\ b1 *) _
+    )
+  | _ |-- (_, _) ---> ([encode (_ - _)], _) =>
+    open_constr:(auto_num_sub
+    (* b0 b1 *) _ _
+    (* env *) _
+    (* s0 s1 s2 *) _ _ _
+    (* x1 x2 *) _ _
+    (* n1 n2 *) _ _
+    (* eval x1 *) _
+    (* eval x2 *) _
+    (* b0 /\ b1 *) _
+    )
+  | _ |-- (_, _) ---> ([encode (_ / _)], _) =>
+    open_constr:(auto_num_div
+    (* b0 b1 *) _ _
+    (* env *) _
+    (* s0 s1 s2 *) _ _ _
+    (* x1 x2 *) _ _
+    (* n1 n2 *) _ _
+    (* eval x1 *) _
+    (* eval x2 *) _
+    (* b0 /\ b1 /\ n2 <> 0 *) _
+    )
+  | _ |-- (_, _) ---> ([encode (if Nat.eqb _ _ then _ else _)], _) =>
+    open_constr:(auto_num_if_eq
+    (* A *) _
+    (* b0 b1 b2 b3 *) _ _ _ _
+    (* env *) _
+    (* s *) _
+    (* x1 x2 y z *) _ _ _ _
+    (* n1 n2 t f *) _ _ _ _
+    (* a *) _
+    (* eval x1 *) _
+    (* eval x2 *) _
+    (* eval y *) _
+    (* eval z *) _
+    (* b0 /\ b1 /\ (if n1 =? n2 then b2 else b3) *) _
+    )
+  end.
+
+Ltac2 doauto () :=
+  match! goal with
+  | [ |- ?g ] =>
+    refine (compile g Lnil); intros
+  end.
+
+Lemma arith_example : forall n,
+  exists prog,
+    Env.empty |-- (prog, empty_state) --->
+    ([encode (letd x := 1 in x + n)], empty_state).
+Proof.
+  intros; eexists.
+  doauto ().
+
+  (* repeat (doauto ()). *)
+
+
+
+  eapply auto_let; intros.
+  all: try (eapply auto_num_add); intros.
+  all: try (eapply auto_num_const); intros.
+  (* all: repeat (autostep; intros). *)
+  all: try eapply trans_Var; try eapply Env.lookup_insert_eq.
+  all: repeat split.
+  all: eauto.
+  - exact I.
+  - exact (fun n : nat => I).
+  Unshelve.
+  exact [].
+  Show Proof.
+  intros; eexists.
+  Opaque encode.
+  repeat (autostep; intros).
+  Show Proof.
+
+  (* eauto with automation. *)
